Setlec/Verify/Deep.lean
@@ -1316,7 +1316,7 @@ theorem iotaRec_WScoped (henv : EnvWF env)
     (h : iotaRec mode (pureFns mode env fuel) env d e = .ok (some e''))
     (hw : WScoped d e) : WScoped d e'' := by
   obtain ⟨c, us, cv, mI, rP, rules, major₀, major₁, major, cj, usj,
-    cvj, cnP, cnF, r, -, -, -, -, -, hfn, hfc, hlen, hmaj, hlit, hsub,
+    cvj, cnP, cnF, r, -, -, -, -, -, hfn, hfc, hlen, -, hmaj, hlit, hsub,
     hmfn, hfj,
     hrule,
     hml, har1, har2, -, hlev, hpeq, hcerts, hmcerts, -, -, -, -, rfl⟩ :=
