Setlec/Verify/InferLeaves.lean
@@ -481,7 +481,7 @@ theorem whnfPres_fvarLeaves {env : Env} (henv : EnvWF env) :
           · exact Or.inr hb
         · -- iota step
           obtain ⟨c, us, cv, mI, rP, rules, major₀, major₁, major, cj, usj,
-            cvj, cnP, cnF, r, -, -, -, -, -, hfn, hfc, hlen, hmaj, hlit,
+            cvj, cnP, cnF, r, -, -, -, -, -, hfn, hfc, hlen, -, hmaj, hlit,
             hsub, hmfn, hfj,
             hrule,
             hml, har1, har2, -, hlev, hpeq, hcerts, hmcerts, -, -, -, -, rfl⟩ :=
@@ -625,7 +625,7 @@ theorem whnfPres_looseBVars {env : Env} (henv : EnvWF env) :
             (looseBVarsBounded_instantiate1_gen hb.2 hbf'.2)
         · -- iota step
           obtain ⟨c, us, cv, mI, rP, rules, major₀, major₁, major, cj, usj,
-            cvj, cnP, cnF, r, -, -, -, -, -, hfn, hfc, hlen, hmaj, hlit,
+            cvj, cnP, cnF, r, -, -, -, -, -, hfn, hfc, hlen, -, hmaj, hlit,
             hsub, hmfn, hfj,
             hrule,
             hml, har1, har2, -, hlev, hpeq, hcerts, hmcerts, -, -, -, -, rfl⟩ :=
